WIP

Clap/Lang/FArray/OneHotRaw.lean
@@ -18,37 +18,55 @@ def runAndEval
   ⟨result, Edsl.CircuitState.eval circuit varStore numAlloc⟩
 
 
-def matchesUnaryBitVecFunctionWithSideEffects
-  {length: ℕ}
-  (p : ℕ)
-  [Fact (p ≥ 2)]
-  (spec_function : (ZMod p) → Vector Bool length)
-  (function : (F p) → Edsl.CircuitStateM p (Vector (FB p) length))
-  (allocates : ℕ)
-: Prop :=
-  ∀ (a : F p) varStorePre numAllocPre,
-  a.isValid (varStorePre.get?) →
-  let a_eval := (a.eval varStorePre.get?).getD 0
-  let ⟨result, numAllocPost, varStorePost, constraints⟩ := runAndEval (function a) numAllocPre varStorePre
-  result.map (FB.toBool · varStorePost.get?) = spec_function a_eval ∧
-  constraints = True ∧
-  numAllocPost = numAllocPre + allocates ∧
-  ∀ i < numAllocPre, varStorePost.get? i = varStorePre.get? i ∧
-  ∀ (i: Fin length),
-    varStorePost.get? (numAllocPost - i) =
-    .some (((spec_function a_eval).get ⟨length - 1 - i, by {
-      omega
-    }⟩).toNat)
+-- def matchesUnaryBitVecFunctionWithSideEffects
+--   {length: ℕ}
+--   (p : ℕ)
+--   [Fact (p ≥ 2)]
+--   (spec_function : (ZMod p) → Vector Bool length)
+--   (function : (F p) → Edsl.CircuitStateM p (Vector (FB p) length))
+--   (allocates : ℕ)
+-- : Prop :=
+--   ∀ (a : F p) varStorePre numAllocPre,
+--   a.isValid (varStorePre.get?) →
+--   let a_eval := (a.eval varStorePre.get?).getD 0
+--   let ⟨result, numAllocPost, varStorePost, constraints⟩ := runAndEval (function a) numAllocPre varStorePre
+--   result.map (FB.toBool · varStorePost.get?) = spec_function a_eval ∧
+--   constraints = True ∧
+--   numAllocPost = numAllocPre + allocates ∧
+--   ∀ i < numAllocPre, varStorePost.get? i = varStorePre.get? i ∧
+--   ∀ (i: Fin length),
+--     varStorePost.get? (numAllocPost - i) =
+--     .some (((spec_function a_eval).get ⟨length - 1 - i, by {
+--       omega
+--     }⟩).toNat)
 
-def spec (p : ℕ) (length : ℕ) [Fact (p ≥ 2)] : Prop := matchesUnaryBitVecFunctionWithSideEffects
+def specFunction (n : ℕ) : Fin n → Vector Bool n := fun i ↦
+  Vector.ofFn λ (idx : Fin n) => idx.val == i
+
+def isValidRange (x : F p) (varStore : ℕ → Option (ZMod p)) : Prop :=
+  let x.eval varStore
+
+instance {k p} [Fact (k ≤ p)] : FB.Convert p (F p) (Fin k) where
+  isValid varStore x := _
+  size := _
+  toLinear := _
+  toIdeal := _
+  toRepresents := _
+  someOfIsValid := _
+  toIdealtoRepresents := _
+  toRepresentstoIdeal := _
+
+def spec (p : ℕ) (length : ℕ) [Fact (p ≥ 2)] : Prop :=
+  Clap.Edsl.Lang.FB.matchesUnaryMonadFunction
   p
-  (Vector.ofFn λ (idx : Fin length) => idx.val = ·)
+  (specFunction length)
   (oneHotRaw length)
   length
 
 lemma equiv (p : ℕ) (length : ℕ) [Fact (p ≥ 2)] :
   spec p length
 := by
+  unfold spec
   intro a varStorePre numAllocPre h_a_isValid
   obtain ⟨a_eval, h_a_eval⟩ := Option.isSome_iff_exists.mp h_a_isValid
   aesop (add simp [
