Clap/Lang/FB/FB.lean
@@ -24,6 +24,29 @@ def toBool (x : FB p) (varStore : ℕ → Option (ZMod p)) : Bool :=
 def ofBool (p : ℕ) [Fact (p ≥ 2)] (x : Bool) : FB p :=
   if x then FB.true p else FB.false p
 
+@[simp, grind .] -- TODO(provisional `simp`)
+lemma eval_ofBool_toBool_of_isValid
+  {p : ℕ}
+  {varStore : ℕ → Option (ZMod p)}
+  (f: FB p)
+  (h : f.isValid varStore)
+  [Fact (p ≥ 2)]
+:
+  (FB.ofBool p (f.toBool varStore)).eval varStore = f.eval varStore
+:= by
+  aesop (add simp [toBool,FB.ofBool,FB.isValid])
+
+@[simp, grind =]
+lemma toBool_ofBool
+  {p : ℕ}
+  {varStore : ℕ → Option (ZMod p)}
+  (b: Bool)
+  [Fact (p ≥ 2)]
+:
+  (FB.ofBool p b).toBool varStore = b
+:= by
+  aesop (add simp [toBool,FB.ofBool,FB.true,FB.false])
+
 namespace ofBool
 
 lemma isAlwaysValid (b:Bool) : isAlwaysValid (FB.ofBool p b) := by
@@ -39,37 +62,131 @@ lemma equiv (varStore) (b) : FixedExp.eval varStore (ofBool p b) =
 
 end ofBool
 
-def matchesUnaryFunction
-  (p : ℕ)
-  [Fact (p ≥ 2)]
-  (spec_function: Bool → Bool)
-  (function : FB p → FB p)
-: Prop :=
-  ∀ (a: FB p) varStore, a.isValid varStore →
-    (function a).eval varStore =
-    (FB.ofBool p (spec_function (a.toBool varStore))).eval varStore
+abbrev withΓ (p : ℕ) (α ω : Type) := (ℕ → Option (ZMod p)) → α → ω
 
-lemma right_inv
-  {p : ℕ}
-  {varStore : ℕ → Option (ZMod p)}
-  (f: FB p)
-  (h : f.isValid varStore)
-  [Fact (p ≥ 2)]
-:
-  (FB.ofBool p (f.toBool varStore)).eval varStore = f.eval varStore
-:= by
-  aesop (add simp [toBool,FB.ofBool,FB.isValid])
+class IsValid (p : ℕ) (α : Type) where
+  isValid : withΓ p α Prop
 
-lemma left_inv
-  {p : ℕ}
-  {varStore : ℕ → Option (ZMod p)}
-  (b: Bool)
-  [Fact (p ≥ 2)]
-:
-  (FB.ofBool p b).toBool varStore = b
-:= by
-  aesop (add simp [toBool,FB.ofBool,FB.true,FB.false])
+def Result (p : ℕ) (α : Type) := α × CircuitResult p
 
+def Result.isPure (result : Result p (ZMod p)) := result.2 = default
+
+/--
+`eval` is allowed to depend on `numAlloc`
+-/
+class Eval (p : ℕ) (α : Type) (β : outParam Type) where
+  eval : ℕ → withΓ p α (Result p β)
+
+instance : Eval p (FB p) (ZMod p) := ⟨fun _numAlloc Γ x ↦ ⟨x.eval Γ |>.getD 0, default⟩⟩
+
+class VarStoreSize (p : ℕ) (α : Type) where
+  size : ℕ
+  toLinear : (ℕ → Option (ZMod p)) → α → Vector (ZMod p) size
+
+class Convert (p : ℕ) (representsT idealT : Type) extends IsValid p representsT, VarStoreSize p representsT where
+  toIdeal : (ℕ → Option (ZMod p)) → representsT → Option idealT
+  toRepresents : idealT → representsT
+  someOfIsValid :
+    ∀ (varStore : ℕ → Option (ZMod p)) (x : representsT),
+      isValid varStore x → (toIdeal varStore x).isSome
+  toIdealtoRepresents :
+    ∀ (varStore : ℕ → Option (ZMod p)) (x : idealT),
+      toIdeal varStore (toRepresents x) = .some x
+  toRepresentstoIdeal :
+    ∀ (varStore : ℕ → Option (ZMod p)) (x : representsT),
+      (h : isValid varStore x) →
+        toIdeal varStore (toRepresents ((toIdeal varStore x).get (someOfIsValid varStore x h))) =
+        toIdeal varStore x
+
+def varStoreSize (p : ℕ) (α : Type) [φ : VarStoreSize p α] : ℕ := φ.size
+
+instance : IsValid p (FB p) := ⟨fun Γ a ↦ FB.isValid a Γ⟩
+
+instance {p} : VarStoreSize p (FB p) where
+  size := 1
+  toLinear varStore x := #v[x.eval varStore |>.getD 42]
+
+instance : Convert p (FB p) Bool where
+  toIdeal Γ x := .some (FB.toBool x Γ)
+  toRepresents := FB.ofBool p
+  someOfIsValid := by simp
+  toIdealtoRepresents := by simp
+  toRepresentstoIdeal := by simp
+
+-- class ΓConsistent (α : Type) where
+--   Γconsistent : ℕ → Prop
+
+-- instance : ΓConsistent (FB )
+
+-- def matchesUnaryBitVecFunctionWithSideEffects
+--   {length: ℕ}
+--   (p : ℕ)
+--   [Fact (p ≥ 2)]
+--   (spec_function : (ZMod p) → Vector Bool length)
+--   (function : (F p) → Edsl.CircuitStateM p (Vector (FB p) length))
+--   (allocates : ℕ)
+-- : Prop :=
+--   ∀ (a : F p) varStorePre numAllocPre,
+--   a.isValid (varStorePre.get?) →
+--   let a_eval := (a.eval varStorePre.get?).getD 0
+--   let ⟨result, numAllocPost, varStorePost, constraints⟩ := runAndEval (function a) numAllocPre varStorePre
+--   result.map (FB.toBool · varStorePost.get?) = spec_function a_eval ∧
+--   constraints = True ∧
+--   numAllocPost = numAllocPre + allocates ∧
+--   ∀ i < numAllocPre, varStorePost.get? i = varStorePre.get? i ∧
+--   ∀ (i: Fin length),
+--     varStorePost.get? (numAllocPost - i) =
+--     .some (((spec_function a_eval).get ⟨length - 1 - i, by {
+--       omega
+--     }⟩).toNat)
+
+open Convert in
+def matchesUnaryFunction (p : ℕ)
+  {funIn funOut specIn specOut : Type}
+  [Convert p funIn specIn] [Convert p funOut specOut]
+  (spec_function : specIn → specOut)
+  (function : funIn → funOut) : Prop :=
+  ∀ (a : funIn) (varStorePre : ℕ → Option (ZMod p)),
+    (h : IsValid.isValid varStorePre a) →
+      letI aVal : specIn := toIdeal varStorePre a |>.get (someOfIsValid _ _ h)
+      letI leftEval : Option specOut := toIdeal varStorePre (function a)
+      letI wrapped : funOut := toRepresents p (spec_function aVal)
+      leftEval = toIdeal varStorePre wrapped
+
+def assertMatchesLast {k} (varStore : ℕ → Option (ZMod p)) (numAlloc : ℕ) (vec : Vector (ZMod p) k) : Prop :=
+  ∀ i < k,
+    letI varStoreIdx := numAlloc - k + i
+    varStore varStoreIdx = vec[i]?
+
+open Convert VarStoreSize in
+def matchesUnaryMonadFunction (p : ℕ)
+  {funIn funOut specIn specOut : Type}
+  [Convert p funIn specIn] [Convert p funOut specOut]
+  (spec_function : specIn → specOut)
+  (function : funIn → CircuitStateM p funOut)
+  (allocatesN : ℕ)
+  (constraints : Prop) : Prop :=
+  ∀ (a : funIn) (varStorePre : Std.ExtTreeMap ℕ (ZMod p)) (numAllocPre : ℕ),
+    (h : IsValid.isValid varStorePre.get? a) →
+      letI aVal : specIn := toIdeal varStorePre.get? a |>.get (someOfIsValid _ _ h)
+      let ⟨result, circuit⟩ : funOut × CircuitResult p :=
+        CircuitStateM.runAndEval (function a) numAllocPre varStorePre
+      let resultIsValid := IsValid.isValid circuit.varStore.get? result
+      letI resultVal : Option specOut := toIdeal circuit.varStore.get? result
+      letI wrapped : funOut := toRepresents p (spec_function aVal)
+      let resultCorrect := resultVal = toIdeal varStorePre.get? wrapped
+      let constraintsCorrect := circuit.constraints = constraints
+      let allocatesCorrect := circuit.numAlloc = numAllocPre + allocatesN
+      let frameRule := ∀ n < numAllocPre, circuit.varStore[n]? = varStorePre[n]?
+      letI resultSize : ℕ := varStoreSize p funOut
+      letI linearRepr := toLinear circuit.varStore.get? result
+      let resultInVarStore := assertMatchesLast circuit.varStore.get? circuit.numAlloc linearRepr
+      resultIsValid ∧
+      resultCorrect ∧
+      constraintsCorrect ∧
+      allocatesCorrect ∧
+      frameRule ∧
+      resultInVarStore
 
 end FB
 
